LambdaDebrujin.v
@@ -1,0 +1,4 @@
+ Inductive LambdaTerm :=
+ | var (v: nat)
+ | app (a b: LambdaTerm)
+ | abst (a: LambdaTerm). 
